Added dis- and mistrust to calculus, reworked to use lists

SecureND.v
@@ -44,6 +44,7 @@ End ATOM.
 (* The resource type, defining the different connectives *)
 Inductive Resource {A: Type} {S: Type}: Type :=
 | nd_atom: A -> Resource
+| nd_bottom: Resource
 | nd_impl: Resource -> Resource -> Resource
 | nd_and: Resource -> Resource -> Resource
 | nd_or: Resource -> Resource -> Resource
@@ -53,12 +54,13 @@ Inductive Resource {A: Type} {S: Type}: Type :=
 | nd_trust: Resource -> Resource.
 
 (* Resources, with equality *)
-Module Resource (R: REPOSITORY) (Atom: ATOM R) <: DecidableType.
+Module RESOURCE (R: REPOSITORY) (Atom: ATOM R) <: DecidableType.
 
   Definition t := @Resource Atom.t R.t.
   Function eq (x y: t): Prop :=
   match x with
   | nd_atom x' => match y with nd_atom y' => Atom.eq x' y' | _ => False end
+  | nd_bottom => match y with nd_bottom => True | _ => False end
   | nd_impl x1 x2 =>
     match y with nd_impl y1 y2 => eq x1 y1 /\ eq x2 y2 | _ => False end
   | nd_and x1 x2 =>
@@ -76,6 +78,7 @@ Module Resource (R: REPOSITORY) (Atom: ATOM R) <: DecidableType.
   Proof.
   induction x;
     first [ apply Atom.eq_refl
+    | reflexivity
     | (split; [apply IHx1 | apply IHx2])
     | apply IHx
     ].
@@ -85,6 +88,7 @@ Module Resource (R: REPOSITORY) (Atom: ATOM R) <: DecidableType.
     intros x y; functional induction eq x y; try (intros; contradiction);
     first
     [ intros Heq; apply Atom.eq_sym; apply Heq
+    | reflexivity
     | intros [H1 H2]; split; [ apply IHP; apply H1 | apply IHP0; apply H2 ]
     | intros H1; apply IHP; apply H1
     ].
@@ -94,6 +98,7 @@ Module Resource (R: REPOSITORY) (Atom: ATOM R) <: DecidableType.
     intros x y; functional induction eq x y; try (intros; contradiction);
     first
     [ destruct z; try (intros; contradiction); intros XY YZ; apply Atom.eq_trans with y'; [ apply XY | apply YZ ]
+    | intros z _ H; apply H
     | destruct z; try (intros; contradiction); intros XY YZ; split; [ apply IHP | apply IHP0 ]; first [ apply XY | apply YZ ]
     | destruct z; try (intros; contradiction); intros XY YZ; apply IHP; [ apply XY | apply YZ ]
     ].
@@ -113,42 +118,103 @@ Module Resource (R: REPOSITORY) (Atom: ATOM R) <: DecidableType.
     | right; intro H; first [ apply Hneq1 | apply Hneq2 ]; apply H
     ].
   Qed.
-End Resource.
+End RESOURCE.
 
-(* A protocol is a set of resources *)
-Module Profile (R: REPOSITORY) (A: ATOM R).
+(* A protocol is a list of resources *)
+(*Module Profile (R: REPOSITORY) (A: ATOM R).
   Module E := Resource(R)(A).  
   Include WSetsOn E.
-End Profile.
+End Profile. *)
 
-(* Define two standard groups Ga and Rb, s.t. Ga < Rb *)
+(* Define two standard repositories Ra and Rb, s.t. Ra < Rb *)
 Declare Module Repository: REPOSITORY.
 Declare Module Atom: ATOM Repository.
-Module Export P := Profile(Repository)(Atom).
+Module Resource := RESOURCE(Repository)(Atom).
+
+(* Module Export P := Profile(Repository)(Atom).
 Module Export PFacts := WFactsOn P.E P.
-Module Export PProps := WPropertiesOn P.E P.
+Module Export PProps := WPropertiesOn P.E P. *)
+
+Axiom resource_eq: forall (a b: Resource.t), Resource.eq a b <-> a = b.
+
+Lemma resource_eq_dec: forall (a b: Resource.t), { a = b } + { a <> b }.
+Proof.
+  intros a b; destruct (Resource.eq_dec a b) as [ Heq | Hneq ];
+  [ left; apply resource_eq; apply Heq
+  | right; intros X; apply Hneq; apply <- resource_eq; apply X
+  ].
+Qed.
+
+Fixpoint profile_eq (Pa: list Resource.t) (Pb: list Resource.t): Prop :=
+  match Pa, Pb with
+  | nil, nil => True
+  | ha::ta, hb::tb => Resource.eq ha hb /\ profile_eq ta tb
+  | _, _ => False
+  end.
+
+Instance profile_eq_equiv: Equivalence profile_eq.
+Proof.
+  split;
+  [ intros P; induction P; 
+    [ simpl; trivial
+    | split; [ reflexivity | apply IHP ]
+    ]
+  | intros Pa; induction Pa; intros Pb; destruct Pb; intros H; try (simpl; trivial); split;
+    [ symmetry; apply (proj1 H)
+    | apply IHPa; apply (proj2 H)
+    ]
+  | intros Pa; induction Pa; intros Pb; destruct Pb; intros Pc; destruct Pc; try (simpl; trivial); try contradiction;
+    intros Hab Hbc; split;
+    [ transitivity t; [ apply (proj1 Hab) | apply (proj1 Hbc) ]
+    | apply IHPa with Pb; [ apply (proj2 Hab) | apply (proj2 Hbc) ]
+    ]
+  ].
+Qed.
+
+Lemma profile_in_eq: forall f Pa Pb, In f Pa -> profile_eq Pa Pb -> In f Pb.
+Proof.
+  intros f Pa; induction Pa; destruct Pb; try contradiction; intros Ha Heq; destruct Ha as [Hf_eq | Hf_in];
+  [ left; transitivity a; [ apply resource_eq; symmetry; apply (proj1 Heq) | apply Hf_eq ]
+  | right; apply IHPa; [ apply Hf_in | apply (proj2 Heq) ]
+  ].
+Qed.
 
 (* typability (of a profile and a message is defined by its properties. *)
-Parameter typable: Repository.t -> P.E.t -> Prop.
+Parameter typable: Repository.t -> Resource.t -> Prop.
 Parameter typable_eq: forall Ra Rb f1 f2,
-  Repository.eq Ra Rb -> P.E.eq f1 f2 -> typable Ra f1 -> typable Rb f2.
-Add Morphism typable with signature Repository.eq ==> P.E.eq ==> Logic.iff as typable_m.
+  Repository.eq Ra Rb -> Resource.eq f1 f2 -> typable Ra f1 -> typable Rb f2.
+Add Morphism typable with signature Repository.eq ==> Resource.eq ==> Logic.iff as typable_m.
 Proof.
-  intros. split.
-    apply typable_eq. apply H. apply H0.
-    apply typable_eq; symmetry; assumption. 
+  intros Ra Rb Hreq a b Hpeq; split; apply typable_eq;
+  [ apply Hreq
+  | apply Hpeq
+  | symmetry; apply Hreq
+  | symmetry; apply Hpeq
+  ].
 Qed.
-  
+
 (* a profile is typable if all its messages are typable *)
-Definition typable_profile (R: Repository.t) (P: P.t): Prop :=
+Definition typable_profile (R: Repository.t) (P: list Resource.t): Prop :=
   forall f, In f P -> typable R f.
-Add Morphism typable_profile with signature Repository.eq ==> P.eq ==> Logic.iff as typable_profile_m.
+
+Lemma typable_sublist: forall R f P, typable_profile R (f::P) -> typable_profile R P.
 Proof.
-  intros. unfold typable_profile. split.
-    intros. apply typable_eq with x f. apply H. reflexivity. apply H1. rewrite H0. apply H2.
-    intros; apply typable_eq with y f. symmetry; assumption. reflexivity. apply H1. rewrite <- H0. apply H2. 
+  intros R f P Htyp x Hin; apply Htyp; right; apply Hin.
 Qed.
-  
+
+Add Morphism typable_profile with signature Repository.eq ==> profile_eq ==> Logic.iff as typable_profile_m.
+Proof.
+  intros Ra Rb Hreq Pa Pb Heq; destruct Pa as [ | a Pa]; destruct Pb as [ | b Pb]; try contradiction;
+  [ split; intros f R Hf; contradiction
+  | split; intros Htyp f [ Hfeq | Hfin ];
+    [ rewrite <- Hfeq; destruct Heq as [Eq_ab Eq_PaPb]; rewrite <- Eq_ab; rewrite <- Hreq; apply Htyp; apply in_eq
+    | destruct Heq as [Eq1 Eq2]; rewrite <- Hreq; apply Htyp; apply in_cons; apply profile_in_eq with Pb; [ apply Hfin | symmetry; apply Eq2 ]
+    | rewrite <- Hfeq; destruct Heq as [Eq_ab Eq_PaPb]; rewrite Eq_ab; rewrite Hreq; apply Htyp; apply in_eq
+    | destruct Heq as [Eq1 Eq2]; rewrite Hreq; apply Htyp; apply in_cons; apply profile_in_eq with Pa; [ apply Hfin | apply Eq2 ]
+    ]
+  ].
+Qed.
+
 (*Lemma dec_and:
   forall P Q, { P } + { ~P } -> { Q } + { ~Q } -> { P /\ Q } + { ~(P /\ Q) }.
 Proof.
@@ -167,12 +233,12 @@ Proof.
     left. exact HnotP.
 Qed.*)
 
-(* wellformedness - this used to include typability, but that is already provided by default *)
-Definition well_formed (P: P.t): Prop :=
-  ~Empty P.
-Add Morphism well_formed with signature P.eq ==> Logic.iff as wf_m.
-  intros Pa Pb Peq; unfold well_formed;
-    split; intros H; [ rewrite <- Peq | rewrite Peq ]; apply H.
+(* wellformedness *)
+Definition well_formed (R: Repository.t) (P: list Resource.t): Prop :=
+  typable_profile R P.
+
+Add Morphism well_formed with signature Repository.eq ==> eq ==> Logic.iff as wf_m.
+  intros Ra Rb Req P; apply typable_profile_m; [ apply Req | reflexivity ].
 Qed.
 
 Section NDC_definition.
@@ -187,90 +253,135 @@ Variable Pb: { x | typable_profile (`Rb) x }.
    (i.e. NDProof P m is a proof of P |- m, where m is a message.)
    The ND calculus
  *)
-Inductive NDProof: list P.t -> P.E.t -> Prop :=
+Inductive NDProof: list Resource.t -> Resource.t -> Prop :=
   | nd_atom_mess: forall b,
       (* well_formed (`Pa) -> *) typable (`Rb) b ->
-      NDProof (`Pa::`Pb::nil) b
+      NDProof (`Pa ++ `Pb) b
   | nd_and_intro: forall f1 f2,
-      NDProof (`Pa::nil) f1 -> typable Ra f1 -> 
-      NDProof (`Pb::nil) f2 -> typable (`Rb) f2 -> 
-      NDProof (`Pa::`Pb::nil) (nd_and f1 f2)
+      NDProof (`Pa) f1 -> typable Ra f1 -> 
+      NDProof (`Pb) f2 -> typable (`Rb) f2 -> 
+      NDProof (`Pa ++ `Pb) (nd_and f1 f2)
   | nd_and_elim_l: forall f1 f2,
-      NDProof (`Pa::`Pb::nil) (nd_and f1 f2) ->
       typable Ra f1 -> typable (`Rb) f2 -> 
-      NDProof (`Pa::`Pb::nil) f1
+      NDProof (`Pa ++ `Pb) (nd_and f1 f2) ->
+      NDProof (`Pa ++ `Pb) f1
   | nd_and_elim_r: forall f1 f2,
-      NDProof (`Pa::`Pb::nil) (nd_and f1 f2) ->
       typable Ra f1 -> typable (`Rb) f2 -> 
-      NDProof (`Pa::`Pb::nil) f2
+      NDProof (`Pa ++ `Pb) (nd_and f1 f2) ->
+      NDProof (`Pa ++ `Pb) f2
   | nd_or_intro_l: forall f1 f2,
-      NDProof (`Pa::`Pb::nil) f1 ->
       typable Ra f1 -> typable (`Rb) f2 -> 
-      NDProof (`Pa::`Pb::nil) (nd_or f1 f2)
+      NDProof (`Pa ++ `Pb) f1 ->
+      NDProof (`Pa ++ `Pb) (nd_or f1 f2)
   | nd_or_intro_r: forall f1 f2,
-      NDProof (`Pa::`Pb::nil) f2 ->
-      typable Ra f1 -> typable (`Rb) f2 -> 
-      NDProof (`Pa::`Pb::nil) (nd_or f1 f2)
+      typable Ra f1 -> typable (`Rb) f2 ->  
+      NDProof (`Pa ++ `Pb) f2 ->
+      NDProof (`Pa ++ `Pb) (nd_or f1 f2)
   | nd_or_elim: forall f1 f2 f, 
-      NDProof (`Pa::`Pb::nil) (nd_or f1 f2) ->
-      typable Ra f1 -> typable (`Rb) f2 -> 
-      NDProof (P.singleton f1::nil) f ->
-      NDProof (P.singleton f2::nil) f ->
-      typable Ra f ->
-      NDProof (`Pa::`Pb::nil) f
+      typable Ra f1 -> typable (`Rb) f2 -> typable Ra f ->
+      NDProof (`Pa ++ `Pb) (nd_or f1 f2) ->
+      NDProof [f1] f ->
+      NDProof [f2] f ->
+      NDProof (`Pa ++ `Pb) f
   | nd_impl_intro: forall f1 f2,
-      NDProof (`Pa::P.singleton f1::nil) f2 ->
       typable (`Rb) f1 -> typable (`Rb) f2 ->
-      NDProof (`Pa::nil) (nd_impl f1 f2)
+      NDProof (`Pa ++ [f1]) f2 ->
+      NDProof (`Pa) (nd_impl f1 f2)
   | nd_impl_elim: forall f1 f2,
-      NDProof (`Pa::nil) (nd_impl f1 f2) ->
       typable (`Rb) f1 -> typable (`Rb) f2 ->
-      NDProof (`Pa::nil) f1 ->
-      NDProof (`Pa::P.singleton f1::nil) f2
+      NDProof (`Pa) (nd_impl f1 f2) ->
+      NDProof (`Pa) f1 ->
+      NDProof (`Pa ++ [f1]) f2
   | nd_read_intro: forall f,
-      well_formed (`Pa) -> typable (`Rb) f ->
-      NDProof (`Pa::nil) (nd_read f)
+      well_formed Ra (`Pa) -> typable (`Rb) f ->
+      NDProof (`Pa) (nd_read f)
   | nd_trust_intro: forall f,
-      NDProof (`Pa::nil) (nd_read f) ->
-      well_formed (P.add f (`Pa)) -> 
-      NDProof (`Pa::nil) (nd_trust f)
+      NDProof (`Pa) (nd_read f) ->
+      well_formed Ra (`Pa ++ [f]) -> 
+      NDProof (`Pa) (nd_trust f)
   | nd_write_intro: forall f,
-      NDProof (`Pa::nil) (nd_read f) -> NDProof (`Pa::nil) (nd_trust f) ->
       typable (`Rb) f ->
-      NDProof (`Pa::nil) (nd_write f).
+      NDProof (`Pa) (nd_read f) ->
+      NDProof (`Pa) (nd_trust f) ->
+      NDProof (`Pa) (nd_write f).
 
-Axiom nd_import: forall f,
+Inductive NDDProof: list Resource.t -> Resource.t -> Prop :=
+  | ndd_normal_proof: forall D f,
+      NDProof D f -> NDDProof D f
+  | nd_bot: forall f1,
+      typable Ra f1 ->
+      NDDProof (`Pa) (nd_impl f1 nd_bottom) ->
+      NDDProof (`Pa) (nd_not f1)
+  | nd_read_distrib: forall f1,
+      typable (`Rb) f1 ->
+      NDDProof (`Pa) (nd_not (nd_read f1)) ->
+      NDDProof (`Pa) (nd_read (nd_not f1))
+  | nd_write_distrib: forall f1,
+      typable (`Rb) f1 ->
+      NDDProof (`Pa) (nd_not (nd_write f1)) ->
+      NDDProof (`Pa) (nd_write (nd_not f1))
+  | nd_trust_distrib: forall f1,
+      typable (`Rb) f1 ->
+      NDDProof (`Pa) (nd_not (nd_trust f1)) ->
+      NDDProof (`Pa) (nd_trust (nd_not f1))
+  | nd_dtrust_intro: forall f1,
+      typable (`Rb) f1 ->
+      well_formed Ra (`Pa) -> NDDProof (`Pa) (nd_impl (nd_read f1) nd_bottom) ->
+      NDDProof (`Pa) (nd_not (nd_trust f1))
+  | nd_dtrust_elim: forall f1 f2,
+      typable (`Rb) f1 -> typable Ra f2 ->
+      NDDProof (`Pa) (nd_not (nd_trust f1)) ->
+      NDDProof (`Pa) (nd_impl (nd_not (nd_trust f1)) f2) ->
+      NDDProof (`Pa) (nd_write f2)
+  | nd_mtrust_intro: forall f1 f2,
+      typable Ra f1 -> typable (`Rb) f2 ->
+      NDDProof (`Pa) (nd_impl (nd_read f2) nd_bottom) ->
+      well_formed Ra (List.remove resource_eq_dec f1 (`Pa)) -> NDDProof [f1] (nd_impl (nd_read f2) nd_bottom) ->
+      NDDProof (List.remove resource_eq_dec f1 (`Pa) ++ [f2]) (nd_not (nd_trust f1))
+  | nd_mtrust_elim1: forall Rc Pc f1 f2,
+      Repository.lt Rc (`Rb) -> typable_profile Rc Pc -> typable Ra f1 -> typable (`Rb) f2 ->
+      NDDProof (List.remove resource_eq_dec f1 (`Pa) ++ [f2]) (nd_not (nd_trust f1)) ->
+      NDDProof (Pc) (nd_impl (nd_read f2) nd_bottom) ->
+      NDDProof (List.remove resource_eq_dec f1 (`Pa) ++ Pc) (nd_trust f2)
+  | nd_mtrust_elim2: forall (Rc: Repository.t | Repository.lt Rc (`Rb))
+      (Pc: list Resource.t | typable_profile (`Rc) Pc) f1 f2,
+      typable Ra f1 -> typable (`Rb) f2 ->
+      NDDProof (List.remove resource_eq_dec f1 (`Pa) ++ [f2]) (nd_not (nd_trust f1)) ->
+      well_formed (`Rb) (`Pc ++ [f2]) ->
+      NDDProof (List.remove resource_eq_dec f1 (`Pa) ++ (`Pc)) (nd_trust f2).
+
+(*Axiom nd_import: forall f,
    NDProof (`Pa::nil) (nd_read f) ->
    typable (`Rb) f ->
-   typable_profile Ra (P.add f (`Pa)).
+   typable_profile Ra (P.add f (`Pa)).*)
 
 (* Properties of dominance *)
 Axiom typable_1_read: forall f,
-  typable Ra f -> NDProof (`Pa::nil) (nd_read f).
+  typable Ra f -> NDProof (`Pa) (nd_read f).
 Axiom typable_1_write: forall f,
-  typable Ra f -> NDProof (`Pa::nil) (nd_write f).
+  typable Ra f -> NDProof (`Pa) (nd_write f).
 Axiom typable_2_read: forall f,
-  typable (`Rb) f -> NDProof (`Pa::nil) (nd_read f).
+  typable (`Rb) f -> NDProof (`Pa) (nd_read f).
 Axiom typable_3_write: forall f,
   typable (`Rb) f ->
-  (NDProof (`Pa::nil) (nd_write f) <->
-     NDProof (`Pa::nil) (nd_read f) /\
-     NDProof (`Pa::nil) (nd_trust f)).
+  (NDProof (`Pa) (nd_write f) <->
+     NDProof (`Pa) (nd_read f) /\
+     NDProof (`Pa) (nd_trust f)).
 
-Axiom proof_in: forall P x,
+(*Axiom proof_in: forall P x,
   NDProof (P::nil) x <-> In x P.
 
 Axiom add_empty_protocol: forall P P' f,
-  NDProof (P::nil) f -> Empty P' -> NDProof (P::P'::nil) f.
+  NDProof (P::nil) f -> Empty P' -> NDProof (P::P'::nil) f.*)
 
 (*Axiom equal_is_okay: forall l1 l2 f,
   NDProof l1 f -> eqlistA eq l1 l2 -> NDProof l2 f.*)
 
-Axiom nd_write_proof: forall R P f, typable_profile R P -> typable R f ->
-  NDProof (P::nil) (nd_write f) -> NDProof (P::nil) f.
+(*Axiom nd_write_proof: forall R P f, typable_profile R P -> typable R f ->
+  NDProof (P::nil) (nd_write f) -> NDProof (P::nil) f.*)
 
 (* Write down version of the import rule *)
-Lemma nd_import_write_down: 
+(*Lemma nd_import_write_down: 
   (forall f, In f (`Pb) -> NDProof (`Pa::nil) (nd_write f)) ->
   well_formed (`Pa) ->
   typable_profile Ra (P.union (`Pa) (`Pb)).
@@ -284,6 +395,6 @@ Proof.
     | | apply add_1; reflexivity
     ]
   ]; apply (proj2_sig Pb); apply Hb.
-Qed.
+Qed.*)
 
 End NDC_definition.
